cleaning up examples

StrataTest/Languages/Boole/array_2d.lean
@@ -2,11 +2,11 @@ import Strata.MetaVerifier
 
 open Strata
 
-private def array2D :=
+private def array_2d :=
 #strata
 program Boole;
 
-procedure array2DWriteRead(i: int, j: int, v: int) returns ()
+procedure array_2d_write_read(i: int, j: int, v: int) returns ()
 {
   var grid : Map int (Map int int);
   grid[i][j] := v;
@@ -15,8 +15,8 @@ procedure array2DWriteRead(i: int, j: int, v: int) returns ()
 
 #end
 
-#eval Strata.Boole.verify "cvc5" array2D
+#eval Strata.Boole.verify "cvc5" array_2d
 
-example : Strata.smtVCsCorrect array2D := by
+example : Strata.smtVCsCorrect array_2d := by
   gen_smt_vcs
   all_goals grind
